oPCF/Syntax.lean
@@ -1,5 +1,9 @@
 import «oPCF».Utility
 
+/-
+The syntax of PCF consists of objects of four sorts: types, contexts, variables, and terms.
+-/
+
 inductive Ty
   | bool
   | nat
@@ -7,27 +11,20 @@ inductive Ty
 
 infixr:100 " ⇒ " => Ty.pow
 
-inductive Ty.is_ground : Ty → Type
-  | bool : bool.is_ground
-  | nat : nat.is_ground
-
 inductive Cx
   | nil
   | cons : Cx -> Ty -> Cx
 
-infixl:100 " ∷ " => Cx.cons
+infixl:70 " ∷ "  => Cx.cons
 
 inductive Var : Cx → Ty → Type
-  | z : Var (Γ ∷ τ) τ
-  | s : ∀ τ, Var Γ τ → Var (Γ ∷ υ) τ
+  | z : ∀ {Γ : Cx}, Var (Γ ∷ τ) τ
+  | s : ∀ {Γ : Cx} {υ : Ty} τ, Var Γ τ → Var (Γ ∷ υ) τ
 
-def Var.succ (x : Var Γ τ) : Var (Γ ∷ υ) τ := s τ x
-
-def Var.tr_cx (t : Var Γ τ) : (Γ = Δ) → (Var Δ τ)
-  | p => by rw [p] at t; exact t
+infix:70 " ∋ " => Var
 
 inductive Tm : Cx → Ty → Type
-  | var : ∀ τ, Var Γ τ → Tm Γ τ
+  | var : ∀ τ, Γ ∋ τ → Tm Γ τ
   | true : Tm Γ .bool
   | false : Tm Γ .bool
   | zero : Tm Γ .nat
@@ -39,19 +36,62 @@ inductive Tm : Cx → Ty → Type
   | app : Tm Γ (τ ⇒ υ) → Tm Γ τ → Tm Γ υ
   | fix : Tm Γ (τ ⇒ τ) → Tm Γ τ
 
-notation:10 Γ " ⊢ " τ => Tm Γ τ
+infix:70 " ⊢ " => Tm
 
-def Var.tm (x : Var Γ τ) : Γ ⊢ τ := Tm.var τ x
+/-
+The types of booleans and naturals are designated as 'ground types'.
+-/
 
-def Tm.from_bool : Bool → (Γ ⊢ .bool)
+inductive Ty.is_ground : Ty → Type
+  | bool : bool.is_ground
+  | nat : nat.is_ground
+
+/-
+We define a notion of appending one context to another. Context appending is associative.
+-/
+
+def Cx.append (Γ : Cx) : Cx → Cx
+  | .nil => Γ
+  | .cons Δ τ => (Γ.append Δ) ∷ τ
+
+instance : Append Cx where
+  append := Cx.append
+
+def Cx.append_assoc (Γ Δ₀ Δ₁ : Cx) : (Γ ++ Δ₀) ++ Δ₁ = Γ ++ (Δ₀ ++ Δ₁) := by
+  induction Δ₁ with
+  | nil => rfl
+  | cons Δ₁ τ Φ => calc ((Γ ++ Δ₀) ++ Δ₁) ∷ τ = (Γ ++ (Δ₀ ++ Δ₁)) ∷ τ := by rw [Φ]
+
+/-
+We also define helper functions for converting terms to variables, weakening variables,
+and casting variables along an identification of contexts.
+-/
+
+def Var.tm (x : Γ ∋ τ) : Γ ⊢ τ := Tm.var τ x
+
+def Var.succ (x : Γ ∋ τ) {υ : Ty} : (Γ ∷ υ) ∋ τ := s τ x
+
+def Var.tr_cx (t : Γ ∋ τ) : (Γ = Δ) → (Δ ∋ τ)
+  | p => by rw [p] at t; exact t
+
+/-
+We define functions for converting booleans and naturals into syntactic booleans and naturals.
+-/
+
+def Tm.from_bool : Bool → Γ ⊢ .bool
   | .true => .true
   | .false => .false
 
-def Tm.from_nat : Nat → (Γ ⊢ .nat)
+def Tm.from_nat : Nat → Γ ⊢ .nat
   | .zero => .zero
   | .succ n => .succ (Tm.from_nat n)
 
-inductive Tm.is_value : (Γ ⊢ τ) → Type
+/-
+Certain terms are designated as 'values'; values of ground type can be converted back to
+mathematical objects of their corresponding type.
+-/
+
+inductive Tm.is_value : Γ ⊢ τ → Type
   | true : true.is_value
   | false : false.is_value
   | zero : zero.is_value
@@ -65,12 +105,3 @@ def Tm.is_value.ground_bool : {v : nil ⊢ .bool} → v.is_value → (n : Bool) 
 def Tm.is_value.ground_nat : {v : nil ⊢ .nat} → v.is_value → (n : Nat) ×' v = from_nat n
   | .zero, .zero => ⟨.zero, rfl⟩
   | .succ _, .succ v' => let Φ := ground_nat v'; ⟨Φ.fst.succ, congrArg Tm.succ Φ.snd⟩
-
-def Cx.append (Γ : Cx) : Cx → Cx
-  | .nil => Γ
-  | .cons Δ τ => Γ.append Δ ∷ τ
-
-def Cx.append_append_eq (Γ Δ₀ Δ₁ : Cx) : (Γ.append Δ₀).append Δ₁ = Γ.append (Δ₀.append Δ₁) := by
-  induction Δ₁ with
-  | nil => rfl
-  | cons Δ₁ τ Φ => calc ((Γ.append Δ₀).append Δ₁) ∷ τ = Γ.append (Δ₀.append Δ₁) ∷ τ := by rw [Φ]
